iris_heap_lang/derived_laws.v
@@ -15,7 +15,7 @@ From iris.prelude Require Import options.
 with lists of values. *)
 
 Definition array `{!heapGS_gen hlc Σ} (l : loc) (dq : dfrac) (vs : list val) : iProp Σ :=
-  [∗ list] i ↦ v ∈ vs, (l +ₗ i) ↦{dq} v.
+  [∗ listZ] i ↦ v ∈ vs, (l +ₗ i) ↦{dq} v.
 
 (** FIXME: Refactor these notations using custom entries once Coq bug #13654
 has been fixed. *)
@@ -53,21 +53,22 @@ Lemma array_nil l dq : l ↦∗{dq} [] ⊣⊢ emp.
 Proof. by rewrite /array. Qed.
 
 Lemma array_singleton l dq v : l ↦∗{dq} [v] ⊣⊢ l ↦{dq} v.
-Proof. by rewrite /array /= right_id loc_add_0. Qed.
+Proof. by rewrite /array big_sepLZ_singleton loc_add_0. Qed.
 
-Lemma array_app l dq vs ws :
-  l ↦∗{dq} (vs ++ ws) ⊣⊢ l ↦∗{dq} vs ∗ (l +ₗ length vs) ↦∗{dq} ws.
+Lemma array_appZ l dq vs ws :
+  l ↦∗{dq} (vs ++ ws) ⊣⊢ l ↦∗{dq} vs ∗ (l +ₗ lengthZ vs) ↦∗{dq} ws.
 Proof.
-  rewrite /array big_sepL_app.
-  setoid_rewrite Nat2Z.inj_add.
+  rewrite /array big_sepLZ_app.
   by setoid_rewrite loc_add_assoc.
 Qed.
+Lemma array_app l dq vs ws :
+  l ↦∗{dq} (vs ++ ws) ⊣⊢ l ↦∗{dq} vs ∗ (l +ₗ Z.of_nat (length vs)) ↦∗{dq} ws.
+Proof. apply array_appZ. Qed.
 
 Lemma array_cons l dq v vs : l ↦∗{dq} (v :: vs) ⊣⊢ l ↦{dq} v ∗ (l +ₗ 1) ↦∗{dq} vs.
 Proof.
-  rewrite /array big_sepL_cons loc_add_0.
+  rewrite /array big_sepLZ_cons loc_add_0.
   setoid_rewrite loc_add_assoc.
-  setoid_rewrite Nat2Z.inj_succ.
   by setoid_rewrite Z.add_1_l.
 Qed.
 
@@ -76,53 +77,80 @@ Global Instance array_cons_frame l dq v vs R Q :
   Frame false R (l ↦∗{dq} (v :: vs)) Q | 2.
 Proof. by rewrite /Frame array_cons. Qed.
 
-Lemma update_array l dq vs off v :
+Lemma update_arrayZ l dq vs (off : Z) v :
   vs !! off = Some v →
   ⊢ l ↦∗{dq} vs -∗ ((l +ₗ off) ↦{dq} v ∗ ∀ v', (l +ₗ off) ↦{dq} v' -∗ l ↦∗{dq} <[off:=v']>vs).
 Proof.
   iIntros (Hlookup) "Hl".
-  rewrite -[X in (l ↦∗{_} X)%I](take_drop_middle _ off v); last done.
-  iDestruct (array_app with "Hl") as "[Hl1 Hl]".
+  rewrite -[X in (l ↦∗{_} X)%I](takeZ_dropZ_middle _ off v); last done.
+  iDestruct (array_appZ with "Hl") as "[Hl1 Hl]".
   iDestruct (array_cons with "Hl") as "[Hl2 Hl3]".
-  assert (off < length vs) as H by (apply lookup_lt_is_Some; by eexists).
-  rewrite take_length min_l; last by lia. iFrame "Hl2".
+  assert (0 ≤ off < lengthZ vs)%Z as H by (apply lookupZ_lt_is_Some; by eexists).
+  rewrite takeZ_lengthZ Z.min_l; last by lia. rewrite Z.max_l; last by lia. iFrame "Hl2".
   iIntros (w) "Hl2".
   clear Hlookup. assert (<[off:=w]> vs !! off = Some w) as Hlookup.
-  { apply list_lookup_insert. lia. }
-  rewrite -[in (l ↦∗{_} <[off:=w]> vs)%I](take_drop_middle (<[off:=w]> vs) off w Hlookup).
-  iApply array_app. rewrite take_insert; last by lia. iFrame.
-  iApply array_cons. rewrite take_length min_l; last by lia. iFrame.
-  rewrite drop_insert_gt; last by lia. done.
+  { apply list_lookupZ_insertZ. lia. }
+  rewrite -[in (l ↦∗{_} <[off:=w]> vs)%I](takeZ_dropZ_middle (<[off:=w]> vs) off w Hlookup).
+  iApply array_appZ. rewrite takeZ_insertZ; last by lia. iFrame.
+  iApply array_cons. rewrite takeZ_lengthZ Z.min_l; last by lia. rewrite Z.max_l; last by lia. iFrame.
+  rewrite dropZ_insertZ_gt; last by lia. done.
 Qed.
+Lemma update_array l dq vs (off : nat) v :
+  vs !! off = Some v →
+  ⊢ l ↦∗{dq} vs -∗ ((l +ₗ Z.of_nat off) ↦{dq} v ∗ ∀ v', (l +ₗ Z.of_nat off) ↦{dq} v' -∗ l ↦∗{dq} <[off:=v']>vs).
+Proof. intros. setoid_rewrite <-insertZ_of_nat. apply update_arrayZ. rewrite lookupZ_of_nat. done. Qed.
 
 (** * Rules for allocation *)
+Lemma mapsto_seqZ_array l dq v n :
+  ([∗ list] i ∈ seqZ 0 n, (l +ₗ i) ↦{dq} v) -∗
+  l ↦∗{dq} replicateZ n v.
+Proof. rewrite /array. rewrite big_sepLZ_replicateZ_seqZ. done. Qed.
 Lemma mapsto_seq_array l dq v n :
-  ([∗ list] i ∈ seq 0 n, (l +ₗ (i : nat)) ↦{dq} v) -∗
+  ([∗ list] i ∈ seq 0 n, (l +ₗ (Z.of_nat i)) ↦{dq} v) -∗
   l ↦∗{dq} replicate n v.
 Proof.
-  rewrite /array. iInduction n as [|n'] "IH" forall (l); simpl.
-  { done. }
-  iIntros "[$ Hl]". rewrite -fmap_S_seq big_sepL_fmap.
-  setoid_rewrite Nat2Z.inj_succ. setoid_rewrite <-Z.add_1_l.
-  setoid_rewrite <-loc_add_assoc. iApply "IH". done.
+  rewrite seq_seqZ big_sepL_fmap. iIntros "H".
+  iEval replace n with (Z.to_nat (Z.of_nat n)) by lia.
+  iApply mapsto_seqZ_array. iApply (big_sepL_impl with "H").
+  iIntros "!#" (?? Hseq%lookup_seqZ). rewrite Z2Nat.id; last by lia. auto.
+Qed.
+
+Lemma twp_allocNZ s E v n :
+  (0 < n)%Z →
+  [[{ True }]] AllocN (Val $ LitV $ LitInt $ n) (Val v) @ s; E
+  [[{ l, RET LitV (LitLoc l); l ↦∗ replicateZ n v ∗
+         [∗ list] i ∈ seqZ 0 n, meta_token (l +ₗ i) ⊤ }]].
+Proof.
+  iIntros (Hzs Φ) "_ HΦ". iApply twp_allocN_seqZ; [done..|].
+  iIntros (l) "Hlm". iApply "HΦ".
+  iDestruct (big_sepL_sep with "Hlm") as "[Hl $]".
+  by iApply mapsto_seqZ_array.
+Qed.
+Lemma wp_allocNZ s E v n :
+  (0 < n)%Z →
+  {{{ True }}} AllocN (Val $ LitV $ LitInt $ n) (Val v) @ s; E
+  {{{ l, RET LitV (LitLoc l); l ↦∗ replicateZ n v ∗
+         [∗ list] i ∈ seqZ 0 n, meta_token (l +ₗ i) ⊤ }}}.
+Proof.
+  iIntros (? Φ) "_ HΦ". iApply (twp_wp_step with "HΦ").
+  iApply twp_allocNZ; [auto..|]; iIntros (l) "H HΦ". by iApply "HΦ".
 Qed.
 
 Lemma twp_allocN s E v n :
   (0 < n)%Z →
   [[{ True }]] AllocN (Val $ LitV $ LitInt $ n) (Val v) @ s; E
   [[{ l, RET LitV (LitLoc l); l ↦∗ replicate (Z.to_nat n) v ∗
-         [∗ list] i ∈ seq 0 (Z.to_nat n), meta_token (l +ₗ (i : nat)) ⊤ }]].
+         [∗ list] i ∈ seq 0 (Z.to_nat n), meta_token (l +ₗ (Z.of_nat i)) ⊤ }]].
 Proof.
-  iIntros (Hzs Φ) "_ HΦ". iApply twp_allocN_seq; [done..|].
-  iIntros (l) "Hlm". iApply "HΦ".
-  iDestruct (big_sepL_sep with "Hlm") as "[Hl $]".
-  by iApply mapsto_seq_array.
+  iIntros (? Φ) "_ HΦ". iApply twp_allocNZ; [done..|].
+  iIntros (l) "[Hl Hmeta]". iApply "HΦ". iFrame "Hl".
+  rewrite seqZ_seq; last by lia. rewrite big_sepL_fmap. done.
 Qed.
 Lemma wp_allocN s E v n :
   (0 < n)%Z →
   {{{ True }}} AllocN (Val $ LitV $ LitInt $ n) (Val v) @ s; E
   {{{ l, RET LitV (LitLoc l); l ↦∗ replicate (Z.to_nat n) v ∗
-         [∗ list] i ∈ seq 0 (Z.to_nat n), meta_token (l +ₗ (i : nat)) ⊤ }}}.
+         [∗ list] i ∈ seq 0 (Z.to_nat n), meta_token (l +ₗ (Z.of_nat i)) ⊤ }}}.
 Proof.
   iIntros (? Φ) "_ HΦ". iApply (twp_wp_step with "HΦ").
   iApply twp_allocN; [auto..|]; iIntros (l) "H HΦ". by iApply "HΦ".
@@ -133,7 +161,7 @@ Lemma twp_allocN_vec s E v n :
   [[{ True }]]
     AllocN #n v @ s ; E
   [[{ l, RET #l; l ↦∗ vreplicate (Z.to_nat n) v ∗
-         [∗ list] i ∈ seq 0 (Z.to_nat n), meta_token (l +ₗ (i : nat)) ⊤ }]].
+         [∗ list] i ∈ seq 0 (Z.to_nat n), meta_token (l +ₗ (Z.of_nat i)) ⊤ }]].
 Proof.
   iIntros (Hzs Φ) "_ HΦ". iApply twp_allocN; [ lia | done | .. ].
   iIntros (l) "[Hl Hm]". iApply "HΦ". rewrite vec_to_list_replicate. iFrame.
@@ -143,104 +171,131 @@ Lemma wp_allocN_vec s E v n :
   {{{ True }}}
     AllocN #n v @ s ; E
   {{{ l, RET #l; l ↦∗ vreplicate (Z.to_nat n) v ∗
-         [∗ list] i ∈ seq 0 (Z.to_nat n), meta_token (l +ₗ (i : nat)) ⊤ }}}.
+         [∗ list] i ∈ seq 0 (Z.to_nat n), meta_token (l +ₗ (Z.of_nat i)) ⊤ }}}.
 Proof.
   iIntros (? Φ) "_ HΦ". iApply (twp_wp_step with "HΦ").
   iApply twp_allocN_vec; [auto..|]; iIntros (l) "H HΦ". by iApply "HΦ".
 Qed.
 
 (** * Rules for accessing array elements *)
-Lemma twp_load_offset s E l dq off vs v :
+Lemma twp_load_offsetZ s E l dq (off : Z) vs v :
   vs !! off = Some v →
   [[{ l ↦∗{dq} vs }]] ! #(l +ₗ off) @ s; E [[{ RET v; l ↦∗{dq} vs }]].
 Proof.
   iIntros (Hlookup Φ) "Hl HΦ".
-  iDestruct (update_array l _ _ _ _ Hlookup with "Hl") as "[Hl1 Hl2]".
+  iDestruct (update_arrayZ l _ _ _ _ Hlookup with "Hl") as "[Hl1 Hl2]".
   iApply (twp_load with "Hl1"). iIntros "Hl1". iApply "HΦ".
-  iDestruct ("Hl2" $! v) as "Hl2". rewrite list_insert_id; last done.
+  iDestruct ("Hl2" $! v) as "Hl2". rewrite list_insertZ_id; last done.
   iApply "Hl2". iApply "Hl1".
 Qed.
-Lemma wp_load_offset s E l dq off vs v :
+Lemma wp_load_offsetZ s E l dq (off : Z) vs v :
   vs !! off = Some v →
   {{{ ▷ l ↦∗{dq} vs }}} ! #(l +ₗ off) @ s; E {{{ RET v; l ↦∗{dq} vs }}}.
 Proof.
   iIntros (? Φ) ">H HΦ". iApply (twp_wp_step with "HΦ").
-  iApply (twp_load_offset with "H"); [by eauto..|]; iIntros "H HΦ".
+  iApply (twp_load_offsetZ with "H"); [by eauto..|]; iIntros "H HΦ".
   by iApply "HΦ".
 Qed.
 
+Lemma twp_load_offset s E l dq (off : nat) vs v :
+  vs !! off = Some v →
+  [[{ l ↦∗{dq} vs }]] ! #(l +ₗ Z.of_nat off) @ s; E [[{ RET v; l ↦∗{dq} vs }]].
+Proof. rewrite -lookupZ_of_nat. apply twp_load_offsetZ. Qed.
+Lemma wp_load_offset s E l dq (off : nat) vs v :
+  vs !! off = Some v →
+  {{{ ▷ l ↦∗{dq} vs }}} ! #(l +ₗ Z.of_nat off) @ s; E {{{ RET v; l ↦∗{dq} vs }}}.
+Proof. rewrite -lookupZ_of_nat. apply wp_load_offsetZ. Qed.
+
 Lemma twp_load_offset_vec s E l dq sz (off : fin sz) (vs : vec val sz) :
-  [[{ l ↦∗{dq} vs }]] ! #(l +ₗ off) @ s; E [[{ RET vs !!! off; l ↦∗{dq} vs }]].
+  [[{ l ↦∗{dq} vs }]] ! #(l +ₗ Z.of_nat off) @ s; E [[{ RET vs !!! off; l ↦∗{dq} vs }]].
 Proof. apply twp_load_offset. by apply vlookup_lookup. Qed.
 Lemma wp_load_offset_vec s E l dq sz (off : fin sz) (vs : vec val sz) :
-  {{{ ▷ l ↦∗{dq} vs }}} ! #(l +ₗ off) @ s; E {{{ RET vs !!! off; l ↦∗{dq} vs }}}.
+  {{{ ▷ l ↦∗{dq} vs }}} ! #(l +ₗ Z.of_nat off) @ s; E {{{ RET vs !!! off; l ↦∗{dq} vs }}}.
 Proof. apply wp_load_offset. by apply vlookup_lookup. Qed.
 
-Lemma twp_store_offset s E l off vs v :
+Lemma twp_store_offsetZ s E l (off : Z) vs v :
   is_Some (vs !! off) →
   [[{ l ↦∗ vs }]] #(l +ₗ off) <- v @ s; E [[{ RET #(); l ↦∗ <[off:=v]> vs }]].
 Proof.
   iIntros ([w Hlookup] Φ) "Hl HΦ".
-  iDestruct (update_array l _ _ _ _ Hlookup with "Hl") as "[Hl1 Hl2]".
+  iDestruct (update_arrayZ l _ _ _ _ Hlookup with "Hl") as "[Hl1 Hl2]".
   iApply (twp_store with "Hl1"). iIntros "Hl1".
   iApply "HΦ". iApply "Hl2". iApply "Hl1".
 Qed.
-Lemma wp_store_offset s E l off vs v :
+Lemma wp_store_offsetZ s E l (off : Z) vs v :
   is_Some (vs !! off) →
   {{{ ▷ l ↦∗ vs }}} #(l +ₗ off) <- v @ s; E {{{ RET #(); l ↦∗ <[off:=v]> vs }}}.
 Proof.
   iIntros (? Φ) ">H HΦ". iApply (twp_wp_step with "HΦ").
-  iApply (twp_store_offset with "H"); [by eauto..|]; iIntros "H HΦ".
+  iApply (twp_store_offsetZ with "H"); [by eauto..|]; iIntros "H HΦ".
   by iApply "HΦ".
 Qed.
 
+Lemma twp_store_offset s E l (off : nat) vs v :
+  is_Some (vs !! off) →
+  [[{ l ↦∗ vs }]] #(l +ₗ Z.of_nat off) <- v @ s; E [[{ RET #(); l ↦∗ <[off:=v]> vs }]].
+Proof. rewrite -lookupZ_of_nat -insertZ_of_nat. apply twp_store_offsetZ. Qed.
+Lemma wp_store_offset s E l (off : nat) vs v :
+  is_Some (vs !! off) →
+  {{{ ▷ l ↦∗ vs }}} #(l +ₗ Z.of_nat off) <- v @ s; E {{{ RET #(); l ↦∗ <[off:=v]> vs }}}.
+Proof. rewrite -lookupZ_of_nat -insertZ_of_nat. apply wp_store_offsetZ. Qed.
+
 Lemma twp_store_offset_vec s E l sz (off : fin sz) (vs : vec val sz) v :
-  [[{ l ↦∗ vs }]] #(l +ₗ off) <- v @ s; E [[{ RET #(); l ↦∗ vinsert off v vs }]].
+  [[{ l ↦∗ vs }]] #(l +ₗ Z.of_nat off) <- v @ s; E [[{ RET #(); l ↦∗ vinsert off v vs }]].
 Proof.
   setoid_rewrite vec_to_list_insert. apply twp_store_offset.
   eexists. by apply vlookup_lookup.
 Qed.
 Lemma wp_store_offset_vec s E l sz (off : fin sz) (vs : vec val sz) v :
-  {{{ ▷ l ↦∗ vs }}} #(l +ₗ off) <- v @ s; E {{{ RET #(); l ↦∗ vinsert off v vs }}}.
+  {{{ ▷ l ↦∗ vs }}} #(l +ₗ Z.of_nat off) <- v @ s; E {{{ RET #(); l ↦∗ vinsert off v vs }}}.
 Proof.
   iIntros (Φ) ">H HΦ". iApply (twp_wp_step with "HΦ").
   iApply (twp_store_offset_vec with "H"); [by eauto..|]; iIntros "H HΦ".
   by iApply "HΦ".
 Qed.
 
-Lemma twp_xchg_offset s E l off vs v v' :
+Lemma twp_xchg_offsetZ s E l (off : Z) vs v v' :
   vs !! off = Some v →
   [[{ l ↦∗ vs }]] Xchg #(l +ₗ off) v' @ s; E [[{ RET v; l ↦∗ <[off:=v']> vs }]].
 Proof.
   iIntros (Hlookup Φ) "Hl HΦ".
-  iDestruct (update_array l _ _ _ _ Hlookup with "Hl") as "[Hl1 Hl2]".
+  iDestruct (update_arrayZ l _ _ _ _ Hlookup with "Hl") as "[Hl1 Hl2]".
   iApply (twp_xchg with "Hl1"). iIntros "Hl1".
   iApply "HΦ". iApply "Hl2". iApply "Hl1".
 Qed.
-Lemma wp_xchg_offset s E l off vs v v' :
+Lemma wp_xchg_offsetZ s E l (off : Z) vs v v' :
   vs !! off = Some v →
   {{{ ▷ l ↦∗ vs }}} Xchg #(l +ₗ off) v' @ s; E {{{ RET v; l ↦∗ <[off:=v']> vs }}}.
 Proof.
   iIntros (? Φ) ">H HΦ". iApply (twp_wp_step with "HΦ").
-  iApply (twp_xchg_offset with "H"); [by eauto..|]; iIntros "H HΦ".
+  iApply (twp_xchg_offsetZ with "H"); [by eauto..|]; iIntros "H HΦ".
   by iApply "HΦ".
 Qed.
 
+Lemma twp_xchg_offset s E l (off : nat) vs v v' :
+  vs !! off = Some v →
+  [[{ l ↦∗ vs }]] Xchg #(l +ₗ Z.of_nat off) v' @ s; E [[{ RET v; l ↦∗ <[off:=v']> vs }]].
+Proof. rewrite -lookupZ_of_nat -insertZ_of_nat. apply twp_xchg_offsetZ. Qed.
+Lemma wp_xchg_offset s E l (off : nat) vs v v' :
+  vs !! off = Some v →
+  {{{ ▷ l ↦∗ vs }}} Xchg #(l +ₗ Z.of_nat off) v' @ s; E {{{ RET v; l ↦∗ <[off:=v']> vs }}}.
+Proof. rewrite -lookupZ_of_nat -insertZ_of_nat. apply wp_xchg_offsetZ. Qed.
+
 Lemma twp_xchg_offset_vec s E l sz (off : fin sz) (vs : vec val sz) v :
-  [[{ l ↦∗ vs }]] Xchg #(l +ₗ off) v @ s; E [[{ RET (vs !!! off); l ↦∗ vinsert off v vs }]].
+  [[{ l ↦∗ vs }]] Xchg #(l +ₗ Z.of_nat off) v @ s; E [[{ RET (vs !!! off); l ↦∗ vinsert off v vs }]].
 Proof.
   setoid_rewrite vec_to_list_insert. apply twp_xchg_offset.
   by apply vlookup_lookup.
 Qed.
 Lemma wp_xchg_offset_vec s E l sz (off : fin sz) (vs : vec val sz) v :
-   {{{ ▷ l ↦∗ vs }}} Xchg #(l +ₗ off) v @ s; E {{{ RET (vs !!! off); l ↦∗ vinsert off v vs }}}.
+   {{{ ▷ l ↦∗ vs }}} Xchg #(l +ₗ Z.of_nat off) v @ s; E {{{ RET (vs !!! off); l ↦∗ vinsert off v vs }}}.
 Proof.
   iIntros (Φ) ">H HΦ". iApply (twp_wp_step with "HΦ").
   iApply (twp_xchg_offset_vec with "H"); [by eauto..|]; iIntros "H HΦ".
   by iApply "HΦ".
 Qed.
 
-Lemma twp_cmpxchg_suc_offset s E l off vs v' v1 v2 :
+Lemma twp_cmpxchg_suc_offsetZ s E l (off : Z) vs v' v1 v2 :
   vs !! off = Some v' →
   v' = v1 →
   vals_compare_safe v' v1 →
@@ -249,11 +304,11 @@ Lemma twp_cmpxchg_suc_offset s E l off vs v' v1 v2 :
   [[{ RET (v', #true); l ↦∗ <[off:=v2]> vs }]].
 Proof.
   iIntros (Hlookup ?? Φ) "Hl HΦ".
-  iDestruct (update_array l _ _ _ _ Hlookup with "Hl") as "[Hl1 Hl2]".
+  iDestruct (update_arrayZ l _ _ _ _ Hlookup with "Hl") as "[Hl1 Hl2]".
   iApply (twp_cmpxchg_suc with "Hl1"); [done..|].
   iIntros "Hl1". iApply "HΦ". iApply "Hl2". iApply "Hl1".
 Qed.
-Lemma wp_cmpxchg_suc_offset s E l off vs v' v1 v2 :
+Lemma wp_cmpxchg_suc_offsetZ s E l (off : Z) vs v' v1 v2 :
   vs !! off = Some v' →
   v' = v1 →
   vals_compare_safe v' v1 →
@@ -262,15 +317,32 @@ Lemma wp_cmpxchg_suc_offset s E l off vs v' v1 v2 :
   {{{ RET (v', #true); l ↦∗ <[off:=v2]> vs }}}.
 Proof.
   iIntros (??? Φ) ">H HΦ". iApply (twp_wp_step with "HΦ").
-  iApply (twp_cmpxchg_suc_offset with "H"); [by eauto..|]; iIntros "H HΦ".
+  iApply (twp_cmpxchg_suc_offsetZ with "H"); [by eauto..|]; iIntros "H HΦ".
   by iApply "HΦ".
 Qed.
+
+Lemma twp_cmpxchg_suc_offset s E l (off : nat) vs v' v1 v2 :
+  vs !! off = Some v' →
+  v' = v1 →
+  vals_compare_safe v' v1 →
+  [[{ l ↦∗ vs }]]
+    CmpXchg #(l +ₗ Z.of_nat off) v1 v2 @ s; E
+  [[{ RET (v', #true); l ↦∗ <[off:=v2]> vs }]].
+Proof. rewrite -lookupZ_of_nat -insertZ_of_nat. apply twp_cmpxchg_suc_offsetZ. Qed.
+Lemma wp_cmpxchg_suc_offset s E l (off : nat) vs v' v1 v2 :
+  vs !! off = Some v' →
+  v' = v1 →
+  vals_compare_safe v' v1 →
+  {{{ ▷ l ↦∗ vs }}}
+    CmpXchg #(l +ₗ Z.of_nat off) v1 v2 @ s; E
+  {{{ RET (v', #true); l ↦∗ <[off:=v2]> vs }}}.
+Proof. rewrite -lookupZ_of_nat -insertZ_of_nat. apply wp_cmpxchg_suc_offsetZ. Qed.
 
 Lemma twp_cmpxchg_suc_offset_vec s E l sz (off : fin sz) (vs : vec val sz) v1 v2 :
   vs !!! off = v1 →
   vals_compare_safe (vs !!! off) v1 →
   [[{ l ↦∗ vs }]]
-    CmpXchg #(l +ₗ off) v1 v2 @ s; E
+    CmpXchg #(l +ₗ Z.of_nat off) v1 v2 @ s; E
   [[{ RET (vs !!! off, #true); l ↦∗ vinsert off v2 vs }]].
 Proof.
   intros. setoid_rewrite vec_to_list_insert.
@@ -281,7 +353,7 @@ Lemma wp_cmpxchg_suc_offset_vec s E l sz (off : fin sz) (vs : vec val sz) v1 v2 
   vs !!! off = v1 →
   vals_compare_safe (vs !!! off) v1 →
   {{{ ▷ l ↦∗ vs }}}
-    CmpXchg #(l +ₗ off) v1 v2 @ s; E
+    CmpXchg #(l +ₗ Z.of_nat off) v1 v2 @ s; E
   {{{ RET (vs !!! off, #true); l ↦∗ vinsert off v2 vs }}}.
 Proof.
   iIntros (?? Φ) ">H HΦ". iApply (twp_wp_step with "HΦ").
@@ -289,7 +361,7 @@ Proof.
   by iApply "HΦ".
 Qed.
 
-Lemma twp_cmpxchg_fail_offset s E l dq off vs v0 v1 v2 :
+Lemma twp_cmpxchg_fail_offsetZ s E l dq (off : Z) vs v0 v1 v2 :
   vs !! off = Some v0 →
   v0 ≠ v1 →
   vals_compare_safe v0 v1 →
@@ -298,13 +370,13 @@ Lemma twp_cmpxchg_fail_offset s E l dq off vs v0 v1 v2 :
   [[{ RET (v0, #false); l ↦∗{dq} vs }]].
 Proof.
   iIntros (Hlookup HNEq Hcmp Φ) "Hl HΦ".
-  iDestruct (update_array l _ _ _ _ Hlookup with "Hl") as "[Hl1 Hl2]".
+  iDestruct (update_arrayZ l _ _ _ _ Hlookup with "Hl") as "[Hl1 Hl2]".
   iApply (twp_cmpxchg_fail with "Hl1"); first done.
   { destruct Hcmp; by [ left | right ]. }
   iIntros "Hl1". iApply "HΦ". iDestruct ("Hl2" $! v0) as "Hl2".
-  rewrite list_insert_id; last done. iApply "Hl2". iApply "Hl1".
+  rewrite list_insertZ_id; last done. iApply "Hl2". iApply "Hl1".
 Qed.
-Lemma wp_cmpxchg_fail_offset s E l dq off vs v0 v1 v2 :
+Lemma wp_cmpxchg_fail_offsetZ s E l dq (off : Z) vs v0 v1 v2 :
   vs !! off = Some v0 →
   v0 ≠ v1 →
   vals_compare_safe v0 v1 →
@@ -313,15 +385,32 @@ Lemma wp_cmpxchg_fail_offset s E l dq off vs v0 v1 v2 :
   {{{ RET (v0, #false); l ↦∗{dq} vs }}}.
 Proof.
   iIntros (??? Φ) ">H HΦ". iApply (twp_wp_step with "HΦ").
-  iApply (twp_cmpxchg_fail_offset with "H"); [by eauto..|]; iIntros "H HΦ".
+  iApply (twp_cmpxchg_fail_offsetZ with "H"); [by eauto..|]; iIntros "H HΦ".
   by iApply "HΦ".
 Qed.
+
+Lemma twp_cmpxchg_fail_offset s E l dq (off : nat) vs v0 v1 v2 :
+  vs !! off = Some v0 →
+  v0 ≠ v1 →
+  vals_compare_safe v0 v1 →
+  [[{ l ↦∗{dq} vs }]]
+    CmpXchg #(l +ₗ Z.of_nat off) v1 v2 @ s; E
+  [[{ RET (v0, #false); l ↦∗{dq} vs }]].
+Proof. rewrite -lookupZ_of_nat. apply twp_cmpxchg_fail_offsetZ. Qed.
+Lemma wp_cmpxchg_fail_offset s E l dq (off : nat) vs v0 v1 v2 :
+  vs !! off = Some v0 →
+  v0 ≠ v1 →
+  vals_compare_safe v0 v1 →
+  {{{ ▷ l ↦∗{dq} vs }}}
+    CmpXchg #(l +ₗ Z.of_nat off) v1 v2 @ s; E
+  {{{ RET (v0, #false); l ↦∗{dq} vs }}}.
+Proof. rewrite -lookupZ_of_nat. apply wp_cmpxchg_fail_offsetZ. Qed.
 
 Lemma twp_cmpxchg_fail_offset_vec s E l dq sz (off : fin sz) (vs : vec val sz) v1 v2 :
   vs !!! off ≠ v1 →
   vals_compare_safe (vs !!! off) v1 →
   [[{ l ↦∗{dq} vs }]]
-    CmpXchg #(l +ₗ off) v1 v2 @ s; E
+    CmpXchg #(l +ₗ Z.of_nat off) v1 v2 @ s; E
   [[{ RET (vs !!! off, #false); l ↦∗{dq} vs }]].
 Proof.
   intros. apply twp_cmpxchg_fail_offset; [|done..].
@@ -331,35 +420,46 @@ Lemma wp_cmpxchg_fail_offset_vec s E l dq sz (off : fin sz) (vs : vec val sz) v1
   vs !!! off ≠ v1 →
   vals_compare_safe (vs !!! off) v1 →
   {{{ ▷ l ↦∗{dq} vs }}}
-    CmpXchg #(l +ₗ off) v1 v2 @ s; E
+    CmpXchg #(l +ₗ Z.of_nat off) v1 v2 @ s; E
   {{{ RET (vs !!! off, #false); l ↦∗{dq} vs }}}.
 Proof.
   intros. eapply wp_cmpxchg_fail_offset; [|done..].
   by apply vlookup_lookup.
 Qed.
 
-Lemma twp_faa_offset s E l off vs (i1 i2 : Z) :
+Lemma twp_faa_offsetZ s E l (off : Z) vs (i1 i2 : Z) :
   vs !! off = Some #i1 →
   [[{ l ↦∗ vs }]] FAA #(l +ₗ off) #i2 @ s; E
   [[{ RET LitV (LitInt i1); l ↦∗ <[off:=#(i1 + i2)]> vs }]].
 Proof.
   iIntros (Hlookup Φ) "Hl HΦ".
-  iDestruct (update_array l _ _ _ _ Hlookup with "Hl") as "[Hl1 Hl2]".
+  iDestruct (update_arrayZ l _ _ _ _ Hlookup with "Hl") as "[Hl1 Hl2]".
   iApply (twp_faa with "Hl1").
   iIntros "Hl1". iApply "HΦ". iApply "Hl2". iApply "Hl1".
 Qed.
-Lemma wp_faa_offset s E l off vs (i1 i2 : Z) :
+Lemma wp_faa_offsetZ s E l (off : Z) vs (i1 i2 : Z) :
   vs !! off = Some #i1 →
   {{{ ▷ l ↦∗ vs }}} FAA #(l +ₗ off) #i2 @ s; E
   {{{ RET LitV (LitInt i1); l ↦∗ <[off:=#(i1 + i2)]> vs }}}.
 Proof.
   iIntros (? Φ) ">H HΦ". iApply (twp_wp_step with "HΦ").
-  iApply (twp_faa_offset with "H"); [by eauto..|]; iIntros "H HΦ". by iApply "HΦ".
+  iApply (twp_faa_offsetZ with "H"); [by eauto..|]; iIntros "H HΦ". by iApply "HΦ".
 Qed.
+
+Lemma twp_faa_offset s E l (off : nat) vs (i1 i2 : Z) :
+  vs !! off = Some #i1 →
+  [[{ l ↦∗ vs }]] FAA #(l +ₗ Z.of_nat off) #i2 @ s; E
+  [[{ RET LitV (LitInt i1); l ↦∗ <[off:=#(i1 + i2)]> vs }]].
+Proof. rewrite -lookupZ_of_nat -insertZ_of_nat. apply twp_faa_offsetZ. Qed.
+Lemma wp_faa_offset s E l (off : nat) vs (i1 i2 : Z) :
+  vs !! off = Some #i1 →
+  {{{ ▷ l ↦∗ vs }}} FAA #(l +ₗ Z.of_nat off) #i2 @ s; E
+  {{{ RET LitV (LitInt i1); l ↦∗ <[off:=#(i1 + i2)]> vs }}}.
+Proof. rewrite -lookupZ_of_nat -insertZ_of_nat. apply wp_faa_offsetZ. Qed.
 
 Lemma twp_faa_offset_vec s E l sz (off : fin sz) (vs : vec val sz) (i1 i2 : Z) :
   vs !!! off = #i1 →
-  [[{ l ↦∗ vs }]] FAA #(l +ₗ off) #i2 @ s; E
+  [[{ l ↦∗ vs }]] FAA #(l +ₗ Z.of_nat off) #i2 @ s; E
   [[{ RET LitV (LitInt i1); l ↦∗ vinsert off #(i1 + i2) vs }]].
 Proof.
   intros. setoid_rewrite vec_to_list_insert. apply twp_faa_offset.
@@ -367,7 +467,7 @@ Proof.
 Qed.
 Lemma wp_faa_offset_vec s E l sz (off : fin sz) (vs : vec val sz) (i1 i2 : Z) :
   vs !!! off = #i1 →
-  {{{ ▷ l ↦∗ vs }}} FAA #(l +ₗ off) #i2 @ s; E
+  {{{ ▷ l ↦∗ vs }}} FAA #(l +ₗ Z.of_nat off) #i2 @ s; E
   {{{ RET LitV (LitInt i1); l ↦∗ vinsert off #(i1 + i2) vs }}}.
 Proof.
   iIntros (? Φ) ">H HΦ". iApply (twp_wp_step with "HΦ").
