iris_heap_lang/lib/array.v
@@ -4,6 +4,8 @@ From iris.heap_lang Require Export derived_laws.
 From iris.heap_lang Require Import proofmode notation.
 From iris.prelude Require Import options.
 
+Local Open Scope Z_scope.
+
 (** Provides some array utilities:
 
 * [array_free], to deallocate an entire array in one go.
@@ -53,17 +55,17 @@ Section proof.
   Context `{!heapGS_gen hlc Σ}.
 
   Lemma twp_array_free s E l vs (n : Z) :
-    n = length vs →
+    n = lengthZ vs →
     [[{ l ↦∗ vs }]] array_free #l #n @ s; E [[{ RET #(); True }]].
   Proof.
     iIntros (Hlen Φ) "Hl HΦ".
     iInduction vs as [|v vs] "IH" forall (l n Hlen); subst n; wp_rec; wp_pures.
     { iApply "HΦ". done. }
-    iDestruct (array_cons with "Hl") as "[Hv Hl]".
+    iDestruct (array_cons with "Hl") as "[Hv Hl]". rewrite cons_lengthZ.
     wp_free. wp_pures. iApply ("IH" with "[] Hl"); eauto with lia.
   Qed.
   Lemma wp_array_free s E l vs (n : Z) :
-    n = length vs →
+    n = lengthZ vs →
     {{{ l ↦∗ vs }}} array_free #l #n @ s; E {{{ RET #(); True }}}.
   Proof.
     iIntros (? Φ) "H HΦ". iApply (twp_wp_step with "HΦ").
@@ -71,7 +73,7 @@ Section proof.
   Qed.
 
   Lemma twp_array_copy_to stk E (dst src : loc) vdst vsrc dq (n : Z) :
-    Z.of_nat (length vdst) = n → Z.of_nat (length vsrc) = n →
+    lengthZ vdst = n → lengthZ vsrc = n →
     [[{ dst ↦∗ vdst ∗ src ↦∗{dq} vsrc }]]
       array_copy_to #dst #src #n @ stk; E
     [[{ RET #(); dst ↦∗ vsrc ∗ src ↦∗{dq} vsrc }]].
@@ -82,13 +84,13 @@ Section proof.
     { iApply "HΦ". auto with iFrame. }
     iDestruct (array_cons with "Hdst") as "[Hv1 Hdst]".
     iDestruct (array_cons with "Hsrc") as "[Hv2 Hsrc]".
-    wp_load; wp_store.
+    wp_load; wp_store. rewrite cons_lengthZ.
     wp_smart_apply ("IH" with "[%] [%] Hdst Hsrc"); [ lia .. | ].
     iIntros "[Hvdst Hvsrc]".
     iApply "HΦ"; by iFrame.
   Qed.
   Lemma wp_array_copy_to stk E (dst src : loc) vdst vsrc dq (n : Z) :
-    Z.of_nat (length vdst) = n → Z.of_nat (length vsrc) = n →
+    lengthZ vdst = n → lengthZ vsrc = n →
     {{{ dst ↦∗ vdst ∗ src ↦∗{dq} vsrc }}}
       array_copy_to #dst #src #n @ stk; E
     {{{ RET #(); dst ↦∗ vsrc ∗ src ↦∗{dq} vsrc }}}.
@@ -98,7 +100,7 @@ Section proof.
   Qed.
 
   Lemma twp_array_clone stk E l dq vl n :
-    Z.of_nat (length vl) = n →
+    lengthZ vl = n →
     (0 < n)%Z →
     [[{ l ↦∗{dq} vl }]]
       array_clone #l #n @ stk; E
@@ -108,14 +110,14 @@ Section proof.
     wp_lam.
     wp_alloc dst as "Hdst"; first by auto.
     wp_smart_apply (twp_array_copy_to with "[$Hdst $Hvl]").
-    - rewrite replicate_length Z2Nat.id; lia.
+    - rewrite replicateZ_lengthZ; lia.
     - auto.
     - iIntros "[Hdst Hl]".
       wp_pures.
       iApply "HΦ"; by iFrame.
   Qed.
   Lemma wp_array_clone stk E l dq vl n :
-    Z.of_nat (length vl) = n →
+    lengthZ vl = n →
     (0 < n)%Z →
     {{{ l ↦∗{dq} vl }}}
       array_clone #l #n @ stk; E
@@ -126,18 +128,18 @@ Section proof.
   Qed.
 
   Section array_init.
-    Context (Q : nat → val → iProp Σ).
-    Implicit Types (f v : val) (i j : nat).
+    Context (Q : Z → val → iProp Σ).
+    Implicit Types (f v : val).
 
     Local Lemma wp_array_init_loop stk E l i n k f  :
-      n = Z.of_nat (i + k) →
+      n = i + Z.of_nat k →
       {{{
         (l +ₗ i) ↦∗ replicate k #() ∗
-        [∗ list] j ∈ seq i k, WP f #(j : nat) @ stk; E {{ Q j }}
+        [∗ list] (j:Z) ∈ seqZ i (Z.of_nat k), WP f #j @ stk; E {{ Q j }}
       }}}
         array_init_loop #l #i #n f @ stk; E
       {{{ vs, RET #();
-        ⌜ length vs = k ⌝ ∗ (l +ₗ i) ↦∗ vs ∗ [∗ list] j↦v ∈ vs, Q (i + j) v
+        ⌜ length vs = k ⌝ ∗ (l +ₗ i) ↦∗ vs ∗ [∗ listZ] j↦v ∈ vs, Q (i + j) v
       }}}.
     Proof.
       iIntros (Hn Φ) "[Hl Hf] HΦ".
@@ -146,25 +148,27 @@ Section proof.
         wp_pures. iApply ("HΦ" $! []). auto. }
       rewrite bool_decide_eq_false_2; last naive_solver lia.
       iDestruct (array_cons with "Hl") as "[Hl HSl]".
+      rewrite Nat2Z.inj_succ seqZ_succ; last by lia.
       iDestruct "Hf" as "[Hf HSf]".
       wp_smart_apply (wp_wand with "Hf"); iIntros (v) "Hv". wp_store. wp_pures.
       rewrite Z.add_1_r -Nat2Z.inj_succ.
       iApply ("IH" with "[%] [HSl] HSf"); first lia.
-      { by rewrite loc_add_assoc Z.add_1_r -Nat2Z.inj_succ. }
+      { by rewrite loc_add_assoc Z.add_1_r. }
       iIntros "!>" (vs). iDestruct 1 as (<-) "[HSl Hvs]".
       iApply ("HΦ" $! (v :: vs)). iSplit; [naive_solver|]. iSplitL "Hl HSl".
-      - iFrame "Hl". by rewrite loc_add_assoc Z.add_1_r -Nat2Z.inj_succ.
-      - iEval (rewrite /= Nat.add_0_r; setoid_rewrite Nat.add_succ_r). iFrame.
+      - iFrame "Hl". by rewrite loc_add_assoc Z.add_1_r.
+      - rewrite big_sepLZ_cons. rewrite Z.add_0_r. iFrame.
+        setoid_rewrite Z.add_succ_comm. iFrame.
     Qed.
     Local Lemma twp_array_init_loop stk E l i n k f  :
-      n = Z.of_nat (i + k) →
+      n = i + Z.of_nat k →
       [[{
         (l +ₗ i) ↦∗ replicate k #() ∗
-        [∗ list] j ∈ seq i k, WP f #(j : nat) @ stk; E [{ Q j }]
+        [∗ list] (j:Z) ∈ seqZ i (Z.of_nat k), WP f #j @ stk; E [{ Q j }]
       }]]
         array_init_loop #l #i #n f @ stk; E
       [[{ vs, RET #();
-        ⌜ length vs = k ⌝ ∗ (l +ₗ i) ↦∗ vs ∗ [∗ list] j↦v ∈ vs, Q (i + j) v
+        ⌜ length vs = k ⌝ ∗ (l +ₗ i) ↦∗ vs ∗ [∗ listZ] j↦v ∈ vs, Q (i + j) v
       }]].
     Proof.
       iIntros (Hn Φ) "[Hl Hf] HΦ".
@@ -173,103 +177,107 @@ Section proof.
         wp_pures. iApply ("HΦ" $! []). auto. }
       rewrite bool_decide_eq_false_2; last naive_solver lia.
       iDestruct (array_cons with "Hl") as "[Hl HSl]".
+      rewrite Nat2Z.inj_succ seqZ_succ; last by lia.
       iDestruct "Hf" as "[Hf HSf]".
       wp_smart_apply (twp_wand with "Hf"); iIntros (v) "Hv". wp_store. wp_pures.
       rewrite Z.add_1_r -Nat2Z.inj_succ.
       iApply ("IH" with "[%] [HSl] HSf"); first lia.
-      { by rewrite loc_add_assoc Z.add_1_r -Nat2Z.inj_succ. }
+      { by rewrite loc_add_assoc Z.add_1_r. }
       iIntros (vs). iDestruct 1 as (<-) "[HSl Hvs]".
       iApply ("HΦ" $! (v :: vs)). iSplit; [naive_solver|]. iSplitL "Hl HSl".
-      - iFrame "Hl". by rewrite loc_add_assoc Z.add_1_r -Nat2Z.inj_succ.
-      - iEval (rewrite /= Nat.add_0_r; setoid_rewrite Nat.add_succ_r). iFrame.
+      - iFrame "Hl". by rewrite loc_add_assoc Z.add_1_r.
+      - rewrite big_sepLZ_cons. rewrite Z.add_0_r. iFrame.
+        setoid_rewrite Z.add_succ_comm. iFrame.
     Qed.
 
     Lemma wp_array_init stk E n f :
       (0 < n)%Z →
       {{{
-        [∗ list] i ∈ seq 0 (Z.to_nat n), WP f #(i : nat) @ stk; E {{ Q i }}
+        [∗ list] (i:Z) ∈ seqZ 0 n, WP f #i @ stk; E {{ Q i }}
       }}}
         array_init #n f @ stk; E
       {{{ l vs, RET #l;
-        ⌜Z.of_nat (length vs) = n⌝ ∗ l ↦∗ vs ∗ [∗ list] k↦v ∈ vs, Q k v
+        ⌜lengthZ vs = n⌝ ∗ l ↦∗ vs ∗ [∗ listZ] k↦v ∈ vs, Q k v
       }}}.
     Proof.
       iIntros (Hn Φ) "Hf HΦ". wp_lam. wp_alloc l as "Hl"; first done.
-      wp_smart_apply (wp_array_init_loop _ _ _ 0 n (Z.to_nat n) with "[Hl $Hf] [HΦ]").
+      wp_smart_apply (wp_array_init_loop _ _ _ 0 n (Z.to_nat n) with "[Hl Hf] [HΦ]").
       { by rewrite /= Z2Nat.id; last lia. }
-      { by rewrite loc_add_0. }
+      { rewrite loc_add_0 Z2Nat.id; last lia. iFrame. }
       iIntros "!>" (vs). iDestruct 1 as (Hlen) "[Hl Hvs]". wp_pures.
       iApply ("HΦ" $! _ vs). iModIntro. iSplit.
-      { iPureIntro. by rewrite Hlen Z2Nat.id; last lia. }
+      { iPureIntro. lia. }
       rewrite loc_add_0. iFrame.
     Qed.
     Lemma twp_array_init stk E n f :
       (0 < n)%Z →
       [[{
-        [∗ list] i ∈ seq 0 (Z.to_nat n), WP f #(i : nat) @ stk; E [{ Q i }]
+        [∗ list] (i:Z) ∈ seqZ 0 n, WP f #i @ stk; E [{ Q i }]
       }]]
         array_init #n f @ stk; E
       [[{ l vs, RET #l;
-        ⌜Z.of_nat (length vs) = n⌝ ∗ l ↦∗ vs ∗ [∗ list] k↦v ∈ vs, Q k v
+        ⌜lengthZ vs = n⌝ ∗ l ↦∗ vs ∗ [∗ listZ] k↦v ∈ vs, Q k v
       }]].
     Proof.
       iIntros (Hn Φ) "Hf HΦ". wp_lam. wp_alloc l as "Hl"; first done.
-      wp_smart_apply (twp_array_init_loop _ _ _ 0 n (Z.to_nat n) with "[Hl $Hf] [HΦ]").
+      wp_smart_apply (twp_array_init_loop _ _ _ 0 n (Z.to_nat n) with "[Hl Hf] [HΦ]").
       { by rewrite /= Z2Nat.id; last lia. }
-      { by rewrite loc_add_0. }
+      { rewrite loc_add_0 Z2Nat.id; last lia. iFrame. }
       iIntros (vs). iDestruct 1 as (Hlen) "[Hl Hvs]". wp_pures.
       iApply ("HΦ" $! _ vs). iModIntro. iSplit.
-      { iPureIntro. by rewrite Hlen Z2Nat.id; last lia. }
+      { iPureIntro. lia. }
       rewrite loc_add_0. iFrame.
     Qed.
   End array_init.
 
   Section array_init_fmap.
-    Context {A} (g : A → val) (Q : nat → A → iProp Σ).
+    Context {A} (g : A → val) (Q : Z → A → iProp Σ).
     Implicit Types (xs : list A) (f : val).
 
-    Local Lemma big_sepL_exists_eq vs :
-      ([∗ list] k↦v ∈ vs, ∃ x, ⌜v = g x⌝ ∗ Q k x) -∗
-      ∃ xs, ⌜ vs = g <$> xs ⌝ ∗ [∗ list] k↦x ∈ xs, Q k x.
+    Local Lemma big_sepLZ_exists_eq vs :
+      ([∗ listZ] k↦v ∈ vs, ∃ x, ⌜v = g x⌝ ∗ Q k x) -∗
+      ∃ xs, ⌜ vs = g <$> xs ⌝ ∗ [∗ listZ] k↦x ∈ xs, Q k x.
     Proof.
       iIntros "Hvs". iInduction vs as [|v vs] "IH" forall (Q); simpl.
       { iExists []. by auto. }
       iDestruct "Hvs" as "[(%x & -> & Hv) Hvs]".
-      iDestruct ("IH" with "Hvs") as (xs ->) "Hxs".
-      iExists (x :: xs). by iFrame.
+      setoid_rewrite Nat2Z.inj_succ.
+      iDestruct ("IH" $! (λ k x, Q (Z.succ k) x) with "Hvs") as (xs ->) "Hxs".
+      iExists (x :: xs). iSplitR; first done.
+      rewrite big_sepLZ_cons. by iFrame.
     Qed.
 
     Lemma wp_array_init_fmap stk E n f :
       (0 < n)%Z →
       {{{
-        [∗ list] i ∈ seq 0 (Z.to_nat n),
-          WP f #(i : nat) @ stk; E {{ v, ∃ x, ⌜v = g x⌝ ∗ Q i x }}
+        [∗ list] (i:Z) ∈ seqZ 0 n,
+          WP f #i @ stk; E {{ v, ∃ x, ⌜v = g x⌝ ∗ Q i x }}
       }}}
         array_init #n f @ stk; E
       {{{ l xs, RET #l;
-        ⌜Z.of_nat (length xs) = n⌝ ∗ l ↦∗ (g <$> xs) ∗ [∗ list] k↦x ∈ xs, Q k x
+        ⌜lengthZ xs = n⌝ ∗ l ↦∗ (g <$> xs) ∗ [∗ listZ] k↦x ∈ xs, Q k x
       }}}.
     Proof.
       iIntros (Hn Φ) "Hf HΦ". iApply (wp_array_init with "Hf"); first done.
       iIntros "!>" (l vs). iDestruct 1 as (<-) "[Hl Hvs]".
-      iDestruct (big_sepL_exists_eq with "Hvs") as (xs ->) "Hxs".
-      iApply "HΦ". iFrame "Hl Hxs". by rewrite fmap_length.
+      iDestruct (big_sepLZ_exists_eq with "Hvs") as (xs ->) "Hxs".
+      iApply "HΦ". iFrame "Hl Hxs". by rewrite fmap_lengthZ.
     Qed.
     Lemma twp_array_init_fmap stk E n f :
       (0 < n)%Z →
       [[{
-        [∗ list] i ∈ seq 0 (Z.to_nat n),
-          WP f #(i : nat) @ stk; E [{ v, ∃ x, ⌜v = g x⌝ ∗ Q i x }]
+        [∗ list] (i:Z) ∈ seqZ 0 n,
+          WP f #i @ stk; E [{ v, ∃ x, ⌜v = g x⌝ ∗ Q i x }]
       }]]
         array_init #n f @ stk; E
       [[{ l xs, RET #l;
-        ⌜Z.of_nat (length xs) = n⌝ ∗ l ↦∗ (g <$> xs) ∗ [∗ list] k↦x ∈ xs, Q k x
+        ⌜lengthZ xs = n⌝ ∗ l ↦∗ (g <$> xs) ∗ [∗ listZ] k↦x ∈ xs, Q k x
       }]].
     Proof.
       iIntros (Hn Φ) "Hf HΦ". iApply (twp_array_init with "Hf"); first done.
       iIntros (l vs). iDestruct 1 as (<-) "[Hl Hvs]".
-      iDestruct (big_sepL_exists_eq with "Hvs") as (xs ->) "Hxs".
-      iApply "HΦ". iFrame "Hl Hxs". by rewrite fmap_length.
+      iDestruct (big_sepLZ_exists_eq with "Hvs") as (xs ->) "Hxs".
+      iApply "HΦ". iFrame "Hl Hxs". by rewrite fmap_lengthZ.
     Qed.
   End array_init_fmap.
 End proof.
