iris_heap_lang/metatheory.v
@@ -156,10 +156,10 @@ Proof.
     apply map_Forall_insert_2; auto.
     apply lookup_union_Some in Hix; last first.
     { eapply heap_array_map_disjoint;
-        rewrite replicate_length Z2Nat.id; auto with lia. }
-    destruct Hix as [(?&?&?&?&?&[-> Hlt%inj_lt]%lookup_replicate_1)%heap_array_lookup|
+        rewrite replicateZ_lengthZ; auto with lia. }
+    destruct Hix as [(?&?&?&?&?&[-> ?]%lookupZ_replicateZ_1)%heap_array_lookup|
                      [j Hj]%elem_of_map_to_list%elem_of_list_lookup_1].
-    + simplify_eq/=. rewrite !Z2Nat.id in Hlt; eauto with lia.
+    + simplify_eq/=. eauto with lia.
     + apply map_Forall_to_list in Hσ.
       by eapply Forall_lookup in Hσ; eauto; simpl in *.
   - apply map_Forall_to_list, Forall_forall.
